Proof transitivity

HockiKlockiLean/HockiKlockiLean/Inclusion.lean
@@ -1,3 +1,4 @@
+import Mathlib.Data.Prod.Basic
 import Mathlib.Data.Set.Basic
 import Mathlib.Logic.Relation
 
@@ -12,47 +13,48 @@ def DimSetVar : Type := String deriving BEq, Hashable, Repr
 
 abbrev DimSetVarRel : Type := Set (DimSetVar × DimSetVar)
 
-inductive WellFormed (a : Dim) (R : DimSetVarRel) (f : DimSetVar → Set Dim) where
-    | wellFormed : (∀ X Y, (X, Y) ∈ R → a ∈ f X → a ∈ f Y) → WellFormed a R f
-
+inductive WellFormed (a : Dim) (R : DimSetVarRel) (f : DimSetVar → Set Dim) : Prop where
+| wellFormed : (∀ {X Y}, (X, Y) ∈ R → a ∈ f X → a ∈ f Y) → WellFormed a R f
 
 theorem empty_relation_well_formed
     {a : Dim}
-    (f : (DimSetVar → Set Dim))
+    (f : DimSetVar → Set Dim)
     :
     WellFormed a ∅ f
-    := by
-        have h1 : ∀ X Y, (X, Y) ∈ (∅ : DimSetVarRel) → a ∈ f X → a ∈ f Y := by
-            intro x y h2
-            by_contra
-            exact Set.not_mem_empty (x, y) h2
-        exact WellFormed.wellFormed h1
+  := by
+    have h1 : ∀ {X Y}, (X, Y) ∈ (∅ : DimSetVarRel) → a ∈ f X → a ∈ f Y := by
+      intro x y h2
+      by_contra
+      exact Set.not_mem_empty (x, y) h2
+    exact WellFormed.wellFormed h1
 
-
-theorem transitive_relation_well_formed
+theorem transitive_step_well_formed
     {a : Dim}
-    (f : (DimSetVar → Set Dim))
+    (f : DimSetVar → Set Dim)
     (R : DimSetVarRel)
     (wf : WellFormed a R f)
+    {X Y Z : DimSetVar}
     (xy_in_R: (X, Y) ∈ R)
     (yz_in_R: (Y, Z) ∈ R)
-    : WellFormed a (insert (X, Z) R) f
-    := by {
-        have R_wf_proof := match wf with
-            | WellFormed.wellFormed proof => proof
+    :
+    WellFormed a (insert (X, Z) R) f
+  := by
+    have R_wf_proof : (∀ {X Y}, (X, Y) ∈ R → a ∈ f X → a ∈ f Y) := match wf with
+      | WellFormed.wellFormed proof => proof
 
-        have xz_wf : a ∈ f X → a ∈ f Z := by
-            have h_xy := R_wf_proof X Y xy_in_R
-            have h_yz := R_wf_proof Y Z yz_in_R
-            intro a_in_fx
-            exact h_yz (h_xy a_in_fx)
+    have xz_wf : a ∈ f X → a ∈ f Z := by
+      have h_xy := R_wf_proof xy_in_R
+      have h_yz := R_wf_proof yz_in_R
+      intro a_in_fx
+      exact h_yz (h_xy a_in_fx)
 
-        have h1 : (∀ x y, (x, y) ∈ (insert (X, Z) R) → a ∈ f x → a ∈ f y) := by
-            intro x y insert_xz a_in_fx
-            rw [Set.mem_insert_iff] at insert_xz
-            match insert_xz with
-                | Or.inl b => sorry
-                | Or.inr b => exact sorry
-
-        exact WellFormed.wellFormed h1
-    }
+    have h1 : (∀ {x u}, (x, u) ∈ (insert (X, Z) R) → a ∈ f x → a ∈ f u) := by
+      intro x u insert_xz a_in_fx
+      rw [Set.mem_insert_iff] at insert_xz
+      match insert_xz with
+        | Or.inl x_u_eq_X_Z =>
+          simp at x_u_eq_X_Z
+          rw [← x_u_eq_X_Z.left, ← x_u_eq_X_Z.right] at xz_wf
+          exact xz_wf a_in_fx
+        | Or.inr b => exact (R_wf_proof b) a_in_fx
+    exact WellFormed.wellFormed h1
